updated cfg logic

lib/rdl/cfg.rb
@@ -16,6 +16,20 @@ attr_accessor :nodes, :edges
     :begin_with_rescue => 10
   }
 
+  EXPR_TYPE_TO_STR = {
+    EXPR_TYPE[:entry] => "entry",
+    EXPR_TYPE[:begin_main] => "begin_main",
+    EXPR_TYPE[:rescue] => "rescue",
+    EXPR_TYPE[:retry] => "retry",
+    EXPR_TYPE[:done] => "done",
+    EXPR_TYPE[:if_head] => "if_head",
+    EXPR_TYPE[:if_then] => "if_then",
+    EXPR_TYPE[:if_else] => "if_else",
+    EXPR_TYPE[:join] => "join",
+    EXPR_TYPE[:begin_secondary] => "begin_secondary",
+    EXPR_TYPE[:begin_with_rescue] => "begin_with_rescue"
+  }
+
   EXPR_TYPE_TO_STATE = {
     RDL::Graph::EXPR_TYPE[:begin_main]      => :Initial,
     RDL::Graph::EXPR_TYPE[:rescue]          => :Error,
@@ -36,7 +50,14 @@ attr_accessor :nodes, :edges
     @predicates = ""
     @pred_name = []
     @retryable_begin_scopes = []
-    # @counter_set = Set.new # Expr type to count mapping
+    @verify = false
+    @begin_effects = {}
+    @rescue_effects = {}
+    @monotonic_pop_nodes = []
+    @counter = Hash.new # Expr type to count mapping
+    @states = Set.new
+    @retry_on_read = false
+    @correct_retry = false
   end
 
   def add_node(node)
@@ -49,11 +70,31 @@ attr_accessor :nodes, :edges
     push_to_stack(to)
   end
 
+  def retry_on_read?
+    @retry_on_read
+  end
+
+  def get_count(expr_type)
+    @counter[expr_type] = 0 unless @counter[expr_type]
+    @counter[expr_type] += 1
+    @counter[expr_type]
+  end
+
+  def get_monotonic_pop_nodes
+    @monotonic_pop_nodes
+  end
+
+  def remove_first_monotonic_pop_node
+    @monotonic_pop_nodes.shift
+  end
+
   def push_to_stack(bbl)
+    @monotonic_pop_nodes = []
     @stack << bbl
   end
 
   def pop_from_stack
+    @monotonic_pop_nodes.push(@stack.last)
     @stack.pop
   end
 
@@ -74,6 +115,11 @@ attr_accessor :nodes, :edges
     # raise "Invalid node" unless @nodes[to]
     @edges[from] = {} unless @edges[from]
     @edges[from][to] = true
+  end
+
+  def get_graph_node(type)
+    @nodes.each { |n| return n[0] if n[1] == type }
+    return
   end
 
   def get_stack_node(type)
@@ -110,9 +156,17 @@ attr_accessor :nodes, :edges
     @begin_visited_secondary = val
   end
 
+  def verify?
+    @verify
+  end
+
+  def set_verify(val)
+    @verify = val
+  end
+
   def to_s
     str = "CFG Nodes:\n"
-    @nodes.each { |n| str += "#{n}\n\n" }
+    @nodes.each { |n| str += "#{n} :::::------>> #{EXPR_TYPE_TO_STR[n[1]]}\n\n" }
     str += "CFG Edges:\n"
     @edges.each_key { |from|
       @edges[from].each_key { |to|
@@ -176,130 +230,311 @@ attr_accessor :nodes, :edges
     EXPR_TYPE_TO_STATE[node.expr_type]
   end
 
-  def generate_predicate(from_state, to_state, effects)
-    @pred_name.push("TransitionFrom#{from_state}To#{to_state}")
-    pred_str = "predicate TransitionFrom#{from_state}To#{to_state} (v:Variables, v':Variables)\n"
+  def generate_predicate(from_state, to_state, effects, lastop, from_node, to_node)
+    cur_lastop = lastop[1]
+    prev_lastop = lastop[0]
+    
+    # op_name is cur_lastop if it is not nil, else it is prev_lastop
+    op_name = cur_lastop ? cur_lastop : prev_lastop
+    @pred_name.push("TransitionFrom#{from_state}#{from_node.get_count}To#{to_state}#{to_node.get_count}with#{op_name}")
+    @states.add("#{from_state}#{from_node.get_count}")
+    @states.add("#{to_state}#{to_node.get_count}")
+    pred_str = "predicate TransitionFrom#{from_state}#{from_node.get_count}To#{to_state}#{to_node.get_count}with#{op_name} (v:Variables, v':Variables)\n"
     pred_str << "  requires Valid(v)\n{\n"
-    pred_str << "  && v.state == #{from_state}\n"
-    pred_str << "  && v'.state == #{to_state}\n"
-    if effects.include?(:read)
-      pred_str << "  && v'.read == v.read - 1\n"
+    pred_str << "  && v.state == #{from_state}#{from_node.get_count}\n"
+    pred_str << "  && v'.state == #{to_state}#{to_node.get_count}\n"
+
+    # TODO: Count should be based on the number of unique writes in a begin block
+    # if len(effects) > 1, then count should be v.count - len(effects), else v.count - 1
+    if effects.length > 1
+      pred_str << "  && v'.count == v.count - #{effects.length}\n"
     else
-      pred_str << "  && v'.read == v.read\n"
+      pred_str << "  && v'.count == v.count - 1\n"
     end
 
-    if effects.include?(:write)
-      pred_str << "  && v'.write == v.write - 1\n"
-    else
-      pred_str << "  && v'.write == v.write\n"
+    if prev_lastop == nil 
+      pred_str << "  && v.lastop != Write\n"
+    end
+
+    if cur_lastop == nil && prev_lastop != nil
+      if prev_lastop == :read
+        pred_str << "  && v.lastop == Read\n"
+      elsif prev_lastop == :write
+        pred_str << "  && v.lastop == Write\n"
+      end
+      if to_state == :Done
+        pred_str << "  && v'.lastop == None\n"
+      end
+    end
+
+    if cur_lastop == :read
+      pred_str << "  && v'.lastop == Read\n"
+    elsif cur_lastop == :write
+      pred_str << "  && v'.lastop == Write\n"
     end
 
     if to_state == :Done
       pred_str << "  && v'.success == v.success + 1\n"
-      pred_str << "  && v'.success <= 1\n"
     else
       pred_str << "  && v'.success == v.success == 0\n"
     end
-
-    pred_str << "  && (v.write > v.read ==> v.write - v.read <= 1)\n"
 
     pred_str << "}\n\n"
     @predicates << pred_str
     pred_str
   end
 
-  def live_dfs(current_node, from_state = :Initial, visited = {}, effects_so_far = [])
-    if visited[current_node]
-      visited[current_node] += 1
-    else
-      visited[current_node] = 1
-    end
+  def update_lastop(lastop, new_op)
+    lastop[0] = lastop[1]
+    lastop[1] = new_op
+  end
 
-    # puts "Visiting #{current_node} with effects so far: #{effects_so_far}\n"
+  # Visited is a Hash : [from_node, to_node] => Set of effects
+
+  def live_dfs(current_node, from_node, from_state = :Initial, visited = Hash.new, effects = {}, lastop = [nil, nil])
+    # if visited[current_node]
+    #   visited[current_node] += 1
+    # else
+    #   visited[current_node] = 1
+    # end
+
+    # puts "\n******Visiting #{current_node} with effects so far: #{effects}********\n\n"
 
     current_state = get_dafny_state(current_node)
 
     if (current_state && from_state != current_state) || (from_state == :Error && current_state)
-      # puts "Generating predicate from #{from_state} to #{current_state} with effects so far: #{effects_so_far}"
-      # puts "Current Node: #{current_node}\n"
-      puts generate_predicate(from_state, current_state, effects_so_far)
+      
+      visited_key = [from_node, current_node]
+      visited_val = effects
+
+      if visited.include?(visited_key)
+        # check if the effects are in the set
+        # if not the same, then we need to visit the node again
+        if visited[visited_key].include?(visited_val)
+          return
+        else
+          visited[visited_key].add(visited_val)
+        end
+      else
+        visited[visited_key] = Set.new
+        visited[visited_key].add(visited_val)
+      end
+      
+      puts "Generating predicate from #{from_state} to #{current_state} with effects so far: #{effects}"
+      puts "\nFrom Node: #{from_node}, Current Node: #{current_node}\n"
+      # Get the last effect from the effects hash
+      cur_lastop = effects.values.last
+      update_lastop(lastop, cur_lastop)
+
+      puts "Lastop list: #{lastop}\n\n"
+
+      if from_state == :Initial && current_state == :Error
+        if @begin_effects.length > 0
+          puts "Begin effects (should be empty): #{@begin_effects}\n"
+          @begin_effects = {}
+        end
+        effects.each do |sym, effect|
+          base = sym.base.name if sym.is_a?(RDL::Type::GenericType)
+          param = sym.params[0].name if sym.is_a?(RDL::Type::GenericType)
+          if base && param
+            @begin_effects[param] = [base, sym]
+          end
+        end
+        puts "Begin effects: #{@begin_effects}\n"
+      end
+
+      if from_state == :Error 
+        if @rescue_effects.length > 0
+          # puts "Rescue effects (should be empty): #{@rescue_effects}\n"
+          # @rescue_effects = {}
+        end
+        effects.each do |sym, effect|
+          base = sym.base.name if sym.is_a?(RDL::Type::GenericType)
+          param = sym.params[0].name if sym.is_a?(RDL::Type::GenericType)
+          if base && param
+            @rescue_effects[param] = [base, sym]
+          end
+        end
+        puts "Rescue effects: #{@rescue_effects}\n"
+      end
+
+
+      # retry on read logic
+      if from_state == :Error && current_state == :Error
+        # check if the retry is the same err node
+        if from_node.get_count == current_node.get_count && lastop[1] == :read
+          @retry_on_read = true
+        end
+      end
+      if from_state == :Error && current_state == :Initial
+        # check if from_node begin_main and to_node rescue with read effect exists in the visited hash
+        # if it does, then we have a retry on read
+        puts "Checking for retry on read\n"
+        begin_node = get_graph_node(RDL::Graph::EXPR_TYPE[:begin_main])
+        rescue_node = get_graph_node(RDL::Graph::EXPR_TYPE[:rescue])
+        effect_set = visited[[begin_node, rescue_node]]
+        puts "Effect set: #{effect_set}\n"
+        if effect_set && effect_set.any? { |eff| eff.values.include?(:read) }
+          @retry_on_read = true
+        end
+      end
+
+      puts generate_predicate(from_state, current_state, effects, lastop, from_node, current_node)
       from_state = current_state
-      effects_so_far = []
+      from_node = current_node
+      effects = {}
     end
 
-    return if visited[current_node] == 2
+    # return if visited[current_node] == 2
 
-    new_effects = effects_so_far + extract_effect_symbols(current_node.effects)
+    cur_symbols = extract_effect_symbols(current_node.effects) # a hashset
+
+    cur_symbols.each do |sym, effect|
+      if !effects.key?(sym)
+        effects[sym] = effect
+      end
+    end
+
+    # new_effects = effects_so_far + extract_effect_symbols(current_node.effects)
 
     # puts "Visiting #{current_node} with new effects: #{new_effects}\n"
+    
+    if current_state == :Initial # since we can cycle back to the initial state
+      lastop = [nil, nil]
+    end
 
     neighbors = @edges[current_node] || {}
     neighbors.each_key do |next_node|
-      live_dfs(next_node, from_state, visited, new_effects.dup)
+      live_dfs(next_node, from_node, from_state, visited, Marshal.load(Marshal.dump(effects)), lastop.dup)
     end
   end
 
   def extract_effect_symbols(effects_arr)
     # If it is a Union type, check the types array of the Union type and see if it is a VarType
-    # To improve this, make symbols a key-value pair with the obj id as the value
+    # To improve this, make a symbol_dict a key-value pair with the obj id as the value
     # and effect (fine-grained parametric) as the key (effect => obj_id)
-    symbols = []
+    symbols = {}
     
     effects_arr = [effects_arr] unless effects_arr.is_a?(Array)
+    effects_arr = effects_arr.flatten
+
+    # puts "Effects Array: #{effects_arr}\n"
+
     effects_arr.each do |eff|
       if eff.is_a?(RDL::Type::VarType)
-        case eff.name
-        when :open
-          symbols << :write
-        when :close
-          symbols << :read
-        when :write
-          symbols << :write
+        if !symbols.key?(eff)
+          case eff.name
+          when :open
+            symbols[eff] = :write
+          when :close
+            symbols[eff] = :read
+          when :write
+            symbols[eff] = :write
+          end
         end
       end
       if eff.is_a?(RDL::Type::UnionType)
         eff.types.each do |type|
           if type.is_a?(RDL::Type::VarType)
-            case type.name
-            when :open
-              symbols << :write
-            when :close
-              symbols << :read
-            when :write
-              symbols << :write
+            if !symbols.key?(type)
+              case type.name
+              when :open
+                symbols[type] = :write
+              when :close
+                symbols[type] = :read
+              when :write
+                symbols[type] = :write
+              end
             end
           end
         end
       end
       if eff.is_a?(RDL::Type::NominalType)
-        case eff.name
-        when "Write"
-          symbols << :write
-        when "Read"
-          symbols << :read
+        if !symbols.key?(eff)
+          case eff.name
+          when "Write"
+            symbols[eff] = :write
+          when "Read"
+            symbols[eff] = :read
+          end
+        end
+      end
+      # #<RDL::Type::GenericType:0x0000000109df6fd8 
+      # @base=#<RDL::Type::NominalType:0x0000000109d1c608 @name="Write">, 
+      # @params=[#<RDL::Type::NominalType:0x0000000109d1c270 @name="Issue">]>
+      if eff.is_a?(RDL::Type::GenericType)
+        if !symbols.key?(eff)
+          case eff.base.name
+          when "Write"
+            symbols[eff] = :write
+          when "Read"
+            symbols[eff] = :read
+          when "Idem"
+            symbols[eff] = :read
+          end
         end
       end
     end
     symbols
   end
 
+  def compare_effects_begin_rescue
+    # Compare if all the Writes in the Begin block have a corresponding Read in the Rescue block
+    # Read the begin_effects hash and check if the value is a Write, find the corresponding key in the rescue
+    # effects hash and check if it is a Read
+    @begin_effects.each do |key, val|
+      if val[0] == "Write"
+        rescue_val = @rescue_effects[key]
+        if rescue_val.nil? || rescue_val[0] != "Read"
+          return false
+        end
+      end
+    end
+    return true
+  end
+
   def to_dafny
-    live_dfs(@nodes.keys.first)
+    live_dfs(@nodes.keys.first, @nodes.keys.first)
+    success = nil
+    comparison = compare_effects_begin_rescue
+
+    puts "\n-------States------"
+    puts @states
+    puts "-------States------\n"
+
+    if !comparison
+      success = false
+      puts "Success: #{success}"
+      # raise "Write in Begin block does not have a corresponding Read in Rescue block\n"
+      raise "Write-Read mismatch/not found\n"
+    end
+
+    if !retry_on_read?
+      success = false
+      puts "Success: #{success}"
+      # raise "No retry on read. Reads can fail if request does not succeed.\n"
+      raise "No retry on read\n"
+    end
+
+    dafny_states = "datatype State = "
+    @states.each do |state|
+      dafny_states << "| #{state}"
+    end
     
-    dafny_types = "datatype State = Initial | Error | Done\n
+    dafny_types = "\ndatatype LastOp = None | Read | Write\n
+
 datatype Variables = Variables(
-  read:nat,
-  write:nat,
+  count:nat,
   success:nat,
+  lastop:LastOp,
   state:State
 )
 
 predicate Init(v:Variables)
 {
-  && v.state == Initial
-  && v.read > 0
-  && v.write > 0
-  && (v.write > v.read ==> v.write - v.read <= 1)
+  && v.state == Initial1
+  && v.count > 0
+  && v.lastop == None
   && v.success == 0
 }\n\n"
 
@@ -324,26 +559,31 @@ predicate Init(v:Variables)
   exists step :: NextStep(v, v', step)
 }\n\n"
     
-    dafny_valid = "predicate Valid(v:Variables)
+    dafny_valid = "predicate Valid(v:Variables)"
+
+    dafny_valid_temp = ""
+    @states.each do |state|
+      if state != "Done1"
+        dafny_valid_temp << " || v.state == #{state}"  
+      end
+    end
+
+    dafny_valid << "
 {
-    && (v.state == Initial || v.state == Error ==> v.success == 0)
-    && (v.state == Done ==> v.success == 1)
-    && v.write >= 0
-    && v.read >= 0
-    && (v.write > v.read ==> v.write - v.read <= 1)
+    && ((#{dafny_valid_temp}) ==> (v.success == 0))
+    && ((v.state == Done1) ==> (v.success == 1))
 }\n\n"
 
     dafny_valid_transition = "predicate ValidTransition(v:Variables, v':Variables)
 {
-    && v.read - v'.read <= 1
-    && v.write - v'.write <= 1
     && v'.success - v.success <= 1
-    && v.read + v.write > v'.read + v'.write
+    && v.count - v'.count == 1
+    && (v.lastop == Write ==> v'.lastop != Write)
 }\n\n"
 
     dafny_safety = "lemma SafetyProof()
-ensures forall v | Init(v) :: Valid(v)
-ensures forall v, v' | Valid(v) && Next(v, v') && ValidTransition(v,v') :: Valid(v')
+  ensures forall v | Init(v) :: Valid(v)
+  ensures forall v, v' | (Valid(v) && Next(v, v')) :: Valid(v') && (ValidTransition(v,v'))
 {
 }\n\n"
 
@@ -352,7 +592,7 @@ ensures forall v, v' | Valid(v) && Next(v, v') && ValidTransition(v,v') :: Valid
 ghost predicate IsTrace(trace: Trace)
 {
     Init(trace(0)) &&
-    forall i: nat :: Valid(trace(i)) && Next(trace(i), trace(i+1)) ==> Valid(trace(i+1)) && ValidTransition(trace(i), trace(i+1))
+    forall i: nat :: (Valid(trace(i)) && Next(trace(i), trace(i+1)))
 }
 
 lemma SafetyProofTrace(trace: Trace)
@@ -362,24 +602,24 @@ lemma SafetyProofTrace(trace: Trace)
     assert Init(trace(0));
     assert Valid(trace(0));
 
-    assert Valid(trace(0)) && Next(trace(0), trace(1)) ==> Valid(trace(1)) && ValidTransition(trace(0), trace(1));
-    assert Valid(trace(1)) && Next(trace(1), trace(2)) ==> Valid(trace(2)) && ValidTransition(trace(1), trace(2));
+    assert Next(trace(0), trace(1)) ==> Valid(trace(1)) && ValidTransition(trace(0), trace(1));
+    // assert Valid(trace(1)) && Next(trace(1), trace(2)) ==> Valid(trace(2)) && ValidTransition(trace(1), trace(2));
 
     // Inductive step:
     forall i | i >= 0
-        ensures Valid(trace(i)) && Next(trace(i), trace(i+1)) && ValidTransition(trace(i), trace(i+1)) ==> Valid(trace(i+1)) 
+      ensures (Valid(trace(i)) && Next(trace(i), trace(i+1))) ==> (Valid(trace(i+1)) && ValidTransition(trace(i), trace(i+1)))
     {
-        if Valid(trace(i)) && Next(trace(i), trace(i+1)){
-            assert trace(i).success <= 1;
-            if trace(i+1).state == Done {
-                assert trace(i+1).success == 1;
-            }
+      if Valid(trace(i)) && Next(trace(i), trace(i+1)){
+        assert trace(i).success <= 1;
+        if trace(i+1).state == Done1 {
+          assert trace(i+1).success == 1;
         }
-        assert Valid(trace(i)) && Next(trace(i), trace(i+1)) && ValidTransition(trace(i), trace(i+1)) ==> Valid(trace(i+1));
-        if Valid(trace(i)) && Next(trace(i), trace(i+1)) && Valid(trace(i+1)) && ValidTransition(trace(i), trace(i+1)) {
-            assert trace(i).read + trace(i).write > trace(i+1).read + trace(i+1).write; 
-            assert trace(i+1).success <= 1;
-        }
+      }
+      // assert Valid(trace(i)) && Next(trace(i), trace(i+1)) ==> Valid(trace(i+1)) && ValidTransition(trace(i), trace(i+1));
+      // if Valid(trace(i)) && Next(trace(i), trace(i+1)) && Valid(trace(i+1)) && ValidTransition(trace(i), trace(i+1)) {
+      //     assert trace(i).count > trace(i+1).count;
+      //     assert trace(i+1).success <= 1;
+      // }
     }
 }
 
@@ -392,43 +632,53 @@ ghost predicate FairNetwork(trace: Trace)
 
 ghost predicate HasDone(n: nat, trace: Trace)
 {
-    exists n' :: n <= n' && trace(n').state == Done && trace(n').success == 1
+    exists n' :: n <= n' && trace(n').state == Done1 && trace(n').success == 1
 }
 
 lemma LivenessProof(trace: Trace, n: nat)
-        returns (n': nat)
+      returns (n': nat)
     requires IsTrace(trace) && FairNetwork(trace)
     requires Init(trace(n))
     requires forall i: nat :: i >= n ==> (Valid(trace(i)) && Next(trace(i), trace(i+1)))
-    ensures n <= n' && trace(n').state == Done && trace(n').success == 1
+    ensures n <= n' && trace(n').state == Done1 && trace(n').success == 1
 {
-    n' := n;
+      n' := n;
     while true
-        invariant n <= n'
-        invariant (Valid(trace(n)) && Next(trace(n), trace(n+1)))
-        invariant Valid(trace(n')) && Next(trace(n'), trace(n'+1)) && ValidTransition(trace(n'), trace(n'+1)) && Valid(trace(n'+1))
-        decreases if Valid(trace(n')) && Next(trace(n'), trace(n'+1)) && Valid(trace(n'+1)) && ValidTransition(trace(n'), trace(n'+1)) then trace(n').read + trace(n').write else 0
+      invariant n <= n'
+      invariant (Valid(trace(n)) && Next(trace(n), trace(n+1)))
+      invariant Valid(trace(n')) && Next(trace(n'), trace(n'+1)) && ValidTransition(trace(n'), trace(n'+1)) && Valid(trace(n'+1))
+      decreases if Valid(trace(n')) && Next(trace(n'), trace(n'+1)) && Valid(trace(n'+1)) && ValidTransition(trace(n'), trace(n'+1)) then trace(n').count else 0
     {
-        SafetyProofTrace(trace);
-        var prev := trace(n').read + trace(n').write;
-        var prev_n := n';
+      SafetyProofTrace(trace);
+      var prev := trace(n').count;
+      var prev_n := n';
 
-        n' := n' + 1;
+      n' := n' + 1;
 
-        assert (trace(n').read + trace(n').write) < prev;
+      assert trace(n').count < prev;
 
-        if trace(n').state == Done {
-            assert trace(n').success == 1;
-            break;
-        }
+      if trace(n').state == Done1 {
+        assert trace(n').success == 1;
+        break;
+      }
     }
-    assert trace(n').state == Done;
+    assert trace(n').state == Done1;
     assert trace(n').success == 1;
 }\n\n"
 
     # Combine all the dafny code and write it to a file
-    dafny_code = dafny_types + @predicates + dafny_step + dafny_next_step + dafny_next + dafny_valid + dafny_valid_transition + dafny_safety + dafny_liveness
+    dafny_code = dafny_states + dafny_types + @predicates + dafny_step + dafny_next_step + dafny_next + dafny_valid + dafny_valid_transition + dafny_safety + dafny_liveness
     File.open("dafny_code.dfy", "w") { |f| f.write(dafny_code) }
+    
+    # Run the cli command dafny verify dafny_code.dfy
+    success = system("dafny verify dafny_code.dfy")
+    
+    if !success
+      puts "Success: #{success}"
+      raise "Verification failed"
+    end
+    puts "Success: #{success}"
+    
     # puts @predicates
     # puts dafny_code
     # puts "Dafny code written to dafny_code.dfy"
@@ -440,9 +690,14 @@ end
 class RDL::Graph::BasicBlock
   attr_accessor :effects, :expr_type, :counter
 
-  def initialize(effects, expr_type = nil, counter = 0)
-    @effects = effects
+  def initialize(effects, expr_type = nil, counter)
+    if effects.is_a? Array
+      @effects = effects
+    else
+      @effects = [effects]
+    end
     @expr_type = expr_type
+    @counter = counter
   end
 
   def add_effect(effect)
@@ -457,7 +712,11 @@ class RDL::Graph::BasicBlock
     @expr_type
   end
 
+  def get_count
+    @counter
+  end
+
   def to_s
-    "Expr_type: #{RDL::Graph::EXPR_TYPE.key(@expr_type)}\n"
+    "Expr_type: #{RDL::Graph::EXPR_TYPE.key(@expr_type)} :: #{@counter}\n"
   end
 end
