lib/types/core/effects.rb
@@ -1,3 +1,10 @@
 class Read; end
 class Write; end
+RDL.type_params :Write, [:t], :all?
+RDL.type_params :Read, [:t], :all?
+RDL.type_params :Idem, [:t], :all?
+class Issue; end
+class Customer; end
+class Payment; end
+class Event; end
 class Idem < Write; end
