test/test_controlflow.rb
@@ -1,6 +1,7 @@
 require 'minitest/autorun'
 $LOAD_PATH << File.dirname(__FILE__) + '/../lib'
 require 'rdl'
+require 'octokit'
 require 'types/core'
 require 'tempfile'
 
@@ -29,15 +30,48 @@ class TestControlFlow < Minitest::Test
       f = File.open('test')
       1+1
     rescue IOError => e
-      a = 1+1
-      b = f.close rescue retry
-      if f == nil
-        retry
-      end
+      # a = 1+1
+      # b = f.close rescue retry
+      # if f == nil
+      #   retry
+      # end
+      retry
     end
   end
 
+  type Octokit::Client, :create_issue, '(String, String, String) -> Sawyer::Resource [Write<Issue>]'
+  type Octokit::Client, :list_issues, '(String) -> Array<Sawyer::Resource> [Read<Issue>]'
+  type Sawyer::Resource, :title, '() -> String'
+
+  type :create_issue,'(Octokit::Client, String, Integer) -> Sawyer::Resource [Write<Issue>]', typecheck: :later
+  def create_issue(octokit, username, attempts)
+    response = octokit.create_issue("#{username}/test-repo2", 'Test Issue 1', 'This is a test issue')
+    raise "Simulated error" if attempts == 0  
+    response
+  end
+
+  type :safe_create_issue, '(Octokit::Client, String, Integer) -> Sawyer::Resource [Read<Issue> or Write<Issue>]', typecheck: :later
+  def safe_create_issue(octokit, username, attempts)
+      begin
+          puts create_issue(octokit, username, attempts)
+      rescue => e
+          attempts += 1
+          if attempts < 3
+              issues = octokit.list_issues("#{username}/test-repo2") rescue retry
+              if issues.any? { |issue| issue.title == 'Test Issue 1' }
+                  puts "An error occurred: #{e.message}. Issue already exists. No more retries."
+              else
+                  puts "#{attempts} An error occurred: #{e.message}. Retrying..."
+                  retry
+              end
+          else
+              puts "An error occurred: #{e.message}. No more retries."
+          end
+      end
+  end
+
   def test_controlflow
-    RDL.do_typecheck :controlflow
+    # RDL.do_typecheck :controlflow
+    RDL.do_typecheck :later
   end
 end
